Incremental work to do real proofs. Build works and tests passing.

qtesla/code/Hacl.Impl.QTesla.Globals.fst
@@ -14,8 +14,10 @@ open Hacl.Impl.QTesla.Params
 open Hacl.Impl.QTesla.Lemmas
 
 module UI32 = FStar.UInt32
+module UI64 = FStar.UInt64
 module I64 = FStar.Int64
 module I32 = FStar.Int32
+module HS = FStar.HyperStack
 
 #reset-options "--z3rlimit 100 --max_fuel 0 --max_ifuel 0"
 
@@ -42,11 +44,40 @@ let is_elem_i64 (e:I64.t) : GTot bool = let x = I64.v e in is_elem_int x
 
 //#reset-options "--z3rlimit 100 --max_fuel 0 --max_ifuel 0"
 
-type elem = e:elem_base{is_elem e}
+type elem = elem_base
 let is_uelem e = let x = uelem_v e in let q = elem_v params_q in 0 <= x /\ x < q
-type uelem = e:uelem_base{is_uelem e}
+type uelem = uelem_base
 type poly = lbuffer elem params_n
+type poly_pred pred = lbuffer (e:elem{pred e}) params_n
 type poly_k = lbuffer elem (params_k *. params_n)
+type poly_k_pred pred = lbuffer (e:elem{pred e}) (params_k *. params_n)
+
+let is_montgomery (e:elem) = 0 <= elem_v e /\ elem_v e < 2 * elem_v params_q
+let is_corrected (e:elem) = -(elem_v params_q) <= elem_v e /\ elem_v e < elem_v params_q
+let is_sampler_output (e:elem) = let b = pow2 (v params_s_bits-1) in -b <= elem_v e /\ elem_v e < b
+
+(*{:pattern (bget h p i)}*)
+//let is_poly_pred (h:HS.mem) (p:poly) (pred:(elem -> Type0)) (k:nat{k <= v params_k * v params_n}) = forall i . (i < k) ==> (pred (bget h p i))
+
+//let is_poly_montgomery_k (h:HS.mem) (p:poly) = is_poly_pred h p is_montgomery
+//let is_poly_corrected_k (h:HS.mem) (p:poly) = is_poly_pred h p is_corrected
+//let is_poly_sampler_output_k (h:HS.mem) (p:poly) = is_poly_pred h p is_sampler_output
+
+unfold let is_poly_montgomery_i (h:HS.mem) (p:poly) (j:nat{j <= v params_n}) = forall i. {:pattern is_montgomery (bget h p i)} (i < j) ==> is_montgomery (bget h p i)
+unfold let is_poly_corrected_i (h:HS.mem) (p:poly) (j:nat{j <= v params_n}) = forall i. {:pattern is_corrected (bget h p i)} (i < j) ==> is_corrected (bget h p i)
+unfold let is_poly_sampler_output_i (h:HS.mem) (p:poly) (j:nat{j <= v params_n}) = forall i. {:pattern is_sampler_output (bget h p i)} (i < j) ==> is_sampler_output (bget h p i)
+
+unfold let is_poly_k_montgomery_i (h:HS.mem) (p:poly_k) (j:nat{j <= v params_k * v params_n}) = forall i. {:pattern is_montgomery (bget h p i)} (i < j) ==> is_montgomery (bget h p i)
+unfold let is_poly_k_corrected_i (h:HS.mem) (p:poly_k) (j:nat{j <= v params_k * v params_n}) = forall i. {:pattern is_corrected (bget h p i)} (i < j) ==> is_corrected (bget h p i)
+unfold let is_poly_k_sampler_output_i (h:HS.mem) (p:poly_k) (j:nat{j <= v params_k * v params_n}) = forall i. {:pattern is_sampler_output (bget h p i)} (i < j) ==> is_sampler_output (bget h p i)
+
+unfold let is_poly_montgomery (h:HS.mem) (p:poly) = is_poly_montgomery_i h p (v params_n)
+unfold let is_poly_corrected (h:HS.mem) (p:poly) = is_poly_corrected_i h p (v params_n)
+unfold let is_poly_sampler_output (h:HS.mem) (p:poly) = is_poly_sampler_output_i h p (v params_n)
+
+unfold let is_poly_k_montgomery (h:HS.mem) (p:poly_k) = is_poly_k_montgomery_i h p (v params_k * v params_n)
+unfold let is_poly_k_corrected (h:HS.mem) (p:poly_k) = is_poly_k_corrected_i h p (v params_k * v params_n)
+unfold let is_poly_k_sampler_output (h:HS.mem) (p:poly_k) = is_poly_k_sampler_output_i h p (v params_k * v params_n)
 
 val poly_create:
     unit
@@ -75,16 +106,32 @@ val index_poly: p: poly_k -> k: size_t{k <. params_k} -> Stack poly
 let index_poly p k = sub p (k *. params_n) params_n
 
 val reduce:
-    a: I64.t{FStar.Int.fits (I64.v a * I64.v params_qinv) I64.n}
-  -> Tot elem
+    a: I64.t{let q = elem_v params_q in let va = I64.v a in va >= 0 /\ va <= (q-1)*(q-1)}
+  -> Tot (r:elem{is_montgomery r})
 
 let reduce a =
-    let u:I64.t = I64.((a *^ params_qinv) &^ 0xffffffffL) in
-    lemma_logand32_value_max I64.(a *^ params_qinv);
-    lemma_logand32_value_min I64.(a *^ params_qinv);
+    // Patrick says even if this multiplication overflows, the bottom 32 bits, which we then mask off, are still
+    // correct -- as in, if the multiplication were contained in a larger machine integer that could not overflow from
+    // the multiplication of two Int64s, the bottom 32 bits are the same.
+
+    // According to Jonathan, overflow on signed integer types is undefined behavior, even if we know the contents are
+    // nonnegative. But since we know the contents are nonnegative, we instead cast to unsigned types and do the
+    // multiplication which, if it overflows, has a well-defined behavior.
+    [@inline_let] let aUnsigned = FStar.Int.Cast.int64_to_uint64 a in
+    [@inline_let] let params_qinv_unsigned = FStar.Int.Cast.int64_to_uint64 params_qinv in
+    let u:I64.t = FStar.Int.Cast.uint64_to_int64 UI64.((aUnsigned *%^ params_qinv_unsigned) &^ 0xFFFFFFFFuL) in
+    lemma_logand32_value_max UI64.(aUnsigned *%^ params_qinv_unsigned);
+    lemma_logand32_value_min UI64.(aUnsigned *%^ params_qinv_unsigned);
+    assert(I64.v u <= pow2 32 - 1);
     let u:I64.t = I64.(u *^ (elem_to_int64 params_q)) in
+    assert(I64.v u <= (pow2 32 - 1) * elem_v params_q);
     let a:I64.t = I64.(a +^ u) in
-    assume(let result = I64.v I64.(a >>^ 32ul) in let q = elem_v params_q in -q < result /\ result < q);
+    //assume(I64.v I64.(a >>^ 32ul) == I64.v a / pow2 32); 
+    //assume(let result = I64.v I64.(a >>^ 32ul) in let q = elem_v params_q in -q < result /\ result < q);
+    //assume(let result = I64.(a >>^ 32ul) in is_montgomery (int64_to_elem result));
+    assert(0 <= I64.v a);
+    shift_right_value_lemma_int64 a 32ul;
+    assert(is_montgomery (int64_to_elem (I64.(a >>^ 32ul))));
     int64_to_elem I64.(a >>^ 32ul)
 
 val barr_reduce:
@@ -119,3 +166,17 @@ let unsafe_declassify #t us =
     | U32  -> Lib.RawIntTypes.u32_to_UInt32 us
     | U64  -> Lib.RawIntTypes.u64_to_UInt64 us
     | U128 -> Lib.RawIntTypes.u128_to_UInt128 us
+
+let buf = t:buftype & a:Type0 & buffer_t t a 
+[@BigOps.__reduce__] unfold
+noextract let bb (#t:buftype) (#a:Type0) (b:buffer_t t a) : GTot buf = (| t, a, b |)
+[@BigOps.__reduce__] unfold
+let disjoint_buf (b0 b1: buf) =
+  let (| _, _, b0 |) = b0 in
+  let (| _, _, b1 |) = b1 in
+  disjoint b0 b1
+[@BigOps.__reduce__] unfold
+let live_buf (h:HS.mem) (b: buf) =
+  let (| _, _, b |) = b in
+  live h b
+
