qtesla/code/Hacl.Impl.QTesla.Lemmas.fst
@@ -3,6 +3,7 @@ module Hacl.Impl.QTesla.Lemmas
 open FStar.HyperStack
 open FStar.HyperStack.ST
 open FStar.Mul
+open FStar.Int
 
 open LowStar.Buffer
 
@@ -13,24 +14,42 @@ open Lib.ByteBuffer
 open Hacl.Impl.QTesla.Params
 
 module UI32 = FStar.UInt32
+module UI64 = FStar.UInt64
 module I32 = FStar.Int32
 module I64 = FStar.Int64
 
 #reset-options "--z3rlimit 100 --max_fuel 0 --max_ifuel 0"
 
-val lemma_logand32_value_max: x:I64.t -> Lemma
-  (ensures (I64.v I64.(x &^ 0xFFFFFFFFL) <= pow2 32 - 1))
+val my_logand_pos_le: #n:pos{1 < n} -> a:int_t n -> b:int_t n{0 <= b} ->
+  Lemma (0 <= Int.logand a b /\ Int.logand a b <= b)
+let my_logand_pos_le #n a b =
+  UInt.logand_le (to_uint a) (to_uint b)
 
-let lemma_logand32_value_max _ = admit()
+val lemma_logand32_value_max: x:UI64.t -> Lemma
+//  (ensures (I64.v I64.(x &^ 0xFFFFFFFFL) <= pow2 32 - 1))
+  (ensures UI64.v (UI64.logand x 0xFFFFFFFFuL) <= pow2 32 - 1)
 
-val lemma_logand32_value_min: x:I64.t -> Lemma
-  (ensures (I64.v I64.(x &^ 0xFFFFFFFFL) >= 0))
+let lemma_logand32_value_max x = 
+    assert(UI64.v 0xFFFFFFFFuL == pow2 32 - 1);
+    //sign_bit_positive #I64.n (I64.v (I64.logand x 0xFFFFFFFFL));
+    //my_logand_pos_le (I64.v x) (I64.v 0xFFFFFFFFL)
+    UInt.logand_le (UI64.v x) 0xFFFFFFFF
 
-let lemma_logand32_value_min _ = admit()
+val lemma_logand32_value_min: x:UI64.t -> Lemma
+  (ensures (UI64.v (UI64.logand x 0xFFFFFFFFuL) >= 0))
+
+let lemma_logand32_value_min x = UInt.logand_le (UI64.v x) 0xFFFFFFFF
+
+val shift_right_value_lemma_int64: x:I64.t{0 <= I64.v x} -> s:UI32.t{UI32.v s < UI64.n} -> Lemma
+  (ensures I64.v (I64.shift_right x s) = (I64.v x) / pow2 (UI32.v s))
+
+let shift_right_value_lemma_int64 x s =
+  FStar.UInt.shift_right_value_lemma #UI64.n (I64.v x) (UI32.v s)
 
 val elem_product_fits_int64: x:elem_base -> y:elem_base -> GTot bool
 let elem_product_fits_int64 x y = FStar.Int.fits (elem_v x * elem_v y) 64
 
+// TODO (kkane): This lemma isn't actually true. We'll need to replace it where it is as we fix our proofs.
 val lemma_elem_product_fits_int64: x:elem_base -> y:elem_base -> Lemma
   (ensures elem_product_fits_int64 x y /\ FStar.Int.fits (elem_v x * elem_v y * I64.v params_qinv) 64)
 
@@ -44,14 +63,49 @@ val lemma_int32_sar_n_minus_1: x:I32.t -> Lemma
 
 let lemma_int32_sar_n_minus_1 x = admit()
 
-val lemma_int32_bitwise_or: x:I32.t -> Lemma
-  (ensures I32.v (0l ^^ x) == I32.v x /\
-           I32.v ((-1l) ^^ x) == (-1) * I32.v x - 1)
+val lemma_int32_logxor_identities: x:I32.t -> Lemma
+  (ensures I32.v (I32.logxor x 0l) == I32.v x /\
+           I32.v (I32.logxor x (-1l)) == (-1) * (I32.v x) - 1) // (-1) * I32.v x - 1)
 
-let lemma_int32_bitwise_or x = admit()
+//let test (x:I32.t) = assert(Int.logxor (I32.v x) (Int.ones I32.n) == (-1) * I32.v x - 1)
 
+let lemma_int32_logxor_identities x = 
+    nth_lemma (Int.logxor (I32.v x) (Int.zero I32.n)) (Int32.v x);
+    admit()
+    
+val lemma_int32_logor_zero: x:I32.t -> Lemma
+  (ensures I32.(x |^ 0l) == x)
+
+let lemma_int32_logor_zero x = nth_lemma #I32.n (I32.v (I32.logor x (I32.int_to_t (zero I32.n)))) (I32.v x)
+
+val lemma_int32_lognot_zero: x:I32.t -> Lemma
+  (requires I32.v x == FStar.Int.zero I32.n)
+  (ensures I32.v (lognot x) == FStar.Int.ones I32.n)
+
+let lemma_int32_lognot_zero x = nth_lemma (Int.lognot (Int.zero I32.n)) (Int.ones I32.n)
+
+open FStar.UInt
+
+val uint_pow2_minus_one: m:nat{m <= bits U32} -> Tot uint32
+let uint_pow2_minus_one m =
+  FStar.Math.Lemmas.pow2_le_compat (bits U32) m;
+  u32 (pow2 m - 1)
+
+val uint_logand_pow2_minus_one: a:uint32 -> m:pos{m <= bits U32} ->
+  Lemma (0 <= v (Lib.IntTypes.logand a (uint_pow2_minus_one m)) /\
+    v (Lib.IntTypes.logand a (uint_pow2_minus_one m)) <= v (uint_pow2_minus_one m))
+let uint_logand_pow2_minus_one a m = admit()
+  //UInt.logand_le #(numbytes U32) (v a) (v (uint_pow2_minus_one m))
+
+val lemma_shift_left_one_eq_pow2: s:shiftval U32 -> Lemma
+  (ensures v (Lib.IntTypes.shift_left (u32 1) s) == pow2 (v s))
+
+let lemma_shift_left_one_eq_pow2 s = admit()
 (*
 val lemma_logand_value_max: x:I64.t -> n:nat -> Lemma
   (requires (n >= 2 /\ n <= 64 /\ FStar.Int.fits (pow2 n - 1) n))
   (ensures (I64.v I64.(x &^ (I64.int_to_t (pow2 n))) <= pow2 n - 1))
 *)
+
+(*private let lemma_q_log_fact _ : Lemma (ensures pow2 (v params_q_log) < 2 * elem_v params_q) =
+    assert_norm(pow2 (v params_q_log) < 2 * elem_v params_q)*)
